equivalence attributes

src/aexp/type.lean
@@ -31,8 +31,8 @@ protected
 def eq (α₁ : aexp X) (α₂ : aexp X) : Prop :=
   quotient.lift_on₂ α₁ α₂ aeq.id $
     λ e₁ e₂ e₃ e₄ e₁_aeq_e₃ e₂_aeq_e₄, propext $
-      iff.intro (λ e₁_aeq_e₂, aeq.id.trans _ (aeq.id.trans _ (aeq.id.symm _ e₁_aeq_e₃) e₁_aeq_e₂) e₂_aeq_e₄)
-                (λ e₃_aeq_e₄, aeq.id.trans _ e₁_aeq_e₃ (aeq.id.trans _ e₃_aeq_e₄ (aeq.id.symm _ e₂_aeq_e₄)))
+      iff.intro (λ e₁_aeq_e₂, aeq.id.trans (aeq.id.trans (aeq.id.symm e₁_aeq_e₃) e₁_aeq_e₂) e₂_aeq_e₄)
+                (λ e₃_aeq_e₄, aeq.id.trans e₁_aeq_e₃ (aeq.id.trans e₃_aeq_e₄ (aeq.id.symm e₂_aeq_e₄)))
 
 instance decidable_eq : decidable_eq (aexp X) :=
   by apply_instance
